ITree_Deadlock.thy
@@ -15,6 +15,9 @@ lemma stable_deadlock [simp]: "stable deadlock"
 lemma deadlock_trace_to: "deadlock \<midarrow>tr\<leadsto> P \<longleftrightarrow> tr = [] \<and> P = deadlock"
   by (auto simp add: deadlock_def)
 
+lemma deadlock_bind [simp]: "deadlock \<bind> P = deadlock"
+  by (metis (no_types, lifting) deadlock_def run_bind run_empty)
+
 definition deadlock_free :: "('e, 'r) itree \<Rightarrow> bool" where
 "deadlock_free P = (\<forall> tr. \<not> P \<midarrow>tr\<leadsto> deadlock)"
 
