examples/ITree_CSP_Examples.thy
@@ -37,15 +37,17 @@ lemma "echo () \<midarrow>[build\<^bsub>Input\<^esub> 1, build\<^bsub>Output\<^e
   apply (subst echo_def[THEN sym])
   apply (simp)
   apply (rule trace_to_Sil)
-  apply (simp add: inp_def)
+  apply (simp add: inp_in_def)
   apply (subst bind_itree.code)
   oops
 
 definition "buffer = 
   loop (\<lambda> s. 
-      do { i \<leftarrow> inp_in Input [0,1,2,3]; Ret (s @ [i]) }
+      do { i \<leftarrow> inp_in Input {0,1,2,3}; Ret (s @ [i]) }
     \<box> do { guard (length s > 0); outp Output (hd s); Ret (tl s) }
     \<box> do { outp State s; Ret s }
   )"
+
+export_code echo buffer in Haskell module_name CSP_Examples file_prefix CSP_Examples (string_classes) 
 
 end
